cryptis/core/rel_state.v
@@ -6,8 +6,9 @@ Unset Strict Implicit.
 Unset Printing Implicit Defensive.
 
 Inductive state :=
-  | Private (ts : gset term)
+  | Private (t : term)
   | Public (t : term)
+  | Secret
   | Invalid.
 
 Section StateCmra.
@@ -21,11 +22,13 @@ Section StateCmra.
 
   #[local] Instance state_op_instance : Op state := λ s1 s2,
     match s1, s2 with
-    | Private ts1, Private ts2 => Private (ts1 ∪ ts2)
-    | Private ts, Public t | Public t, Private ts =>
-      if bool_decide (ts ⊆ {[ t ]}) then Public t else Invalid
+    | Private t1, Private t2 =>
+      if bool_decide (t1 = t2) then Private t1 else Secret
+    | Private t1, Public t2 | Public t2, Private t1 =>
+      if bool_decide (t1 = t2) then Public t2 else Invalid
     | Public t1, Public t2 =>
       if bool_decide (t1 = t2) then Public t1 else Invalid
+    | Private _, Secret | Secret, Private _ | Secret, Secret => Secret
     | _, _ => Invalid
     end.
 
@@ -37,7 +40,8 @@ Section StateCmra.
     | _ => True
     end.
 
-  #[local] Instance state_unit_instance : Unit state := Private ∅.
+  Lemma state_op st1 st2 : st1 ⋅ st2 = state_op_instance st1 st2.
+  Proof. by []. Qed.
 
   Lemma state_ra_mixin : RAMixin state.
   Proof.
@@ -47,17 +51,13 @@ Section StateCmra.
   - solve_proper.
   - intros [] [] [];
     rewrite /op /state_op_instance;
-    repeat case_bool_decide;
-    try (f_equiv; set_solver);
-    try (exfalso; set_solver).
+    repeat (case_bool_decide; simplify_eq/=); congruence.
   - intros [] [];
     rewrite /op /state_op_instance;
-    repeat case_bool_decide; simplify_eq;
-    f_equiv; set_solver.
+    repeat (case_bool_decide; simplify_eq/=); congruence.
   - intros [] ? [= <-];
     rewrite /op /state_op_instance;
-    repeat case_bool_decide; simplify_eq;
-    f_equiv; set_solver.
+    repeat (case_bool_decide; simplify_eq/=); congruence.
   - by move=> [] [].
   - rewrite /pcore /state_pcore_instance.
     move=> ? ? ? ? H.
@@ -65,17 +65,7 @@ Section StateCmra.
   - by move=> [] [].
   Qed.
 
-  Lemma state_ucmra_mixin : UcmraMixin state.
-  Proof.
-  split=> // s.
-  change (ε ⋅ s) with (state_op_instance ε s).
-  case: s => [ts|t|] //=.
-  + f_equiv; set_solver.
-  + case_bool_decide=> //; set_solver.
-  Qed.
-
   Canonical Structure stateR := discreteR state state_ra_mixin.
-  Canonical Structure stateUR := Ucmra state state_ucmra_mixin.
 
   #[global] Instance stateR_discrete : CmraDiscrete stateR.
   Proof. by split; first apply _. Qed.
@@ -83,46 +73,77 @@ Section StateCmra.
   #[global] Instance state_core_id (st : state) : CoreId st.
   Proof. by constructor. Qed.
 
+  #[global] Instance stateR_total : CmraTotal stateR.
+  Proof. by move=> st; exists st. Qed.
+
+  Lemma Private_included_Public t : Private t ≼ Public t.
+  Proof. exists (Public t). rewrite state_op /=. by case_bool_decide. Qed.
+
+  Lemma Private_included_Secret t : Private t ≼ Secret.
+  Proof. by exists Secret. Qed.
+
+  Lemma Private_included t st :
+    ✓ st → Private t ≼ st → st = Private t ∨ st = Secret ∨ st = Public t.
+  Proof.
+  move=> Hval [z Heq]. fold_leibniz. subst st. move: Hval. rewrite state_op.
+  case: z => [t1|t1||] //=; repeat (case_bool_decide; simplify_eq/=); try done; eauto.
+  Qed.
+
+  Lemma Public_included t st : ✓ st → Public t ≼ st → st = Public t.
+  Proof.
+  move=> Hval [z Heq]. fold_leibniz. subst st. move: Hval. rewrite state_op.
+  case: z => [t1|t1||] //=; repeat (case_bool_decide; simplify_eq/=); try done; eauto.
+  Qed.
+
+  Lemma Secret_included st : ✓ st → Secret ≼ st → st = Secret.
+  Proof.
+  move=> Hval [z Heq]. fold_leibniz. subst st. move: Hval. rewrite state_op. by case: z.
+  Qed.
+
+  Lemma Public_Public_valid t1 t2 : ✓ (Public t1 ⋅ Public t2) → t1 = t2.
+  Proof. rewrite state_op /=. by case_bool_decide. Qed.
+
+  Lemma Private_Public_valid t1 t2 : ✓ (Private t1 ⋅ Public t2) → t1 = t2.
+  Proof. rewrite state_op /=. by case_bool_decide. Qed.
+
+  Lemma Secret_Public_valid t : ✓ (Secret ⋅ Public t) → False.
+  Proof. by rewrite state_op. Qed.
+
 End StateCmra.
 
 Section StateUpdates.
 
   Context {SI : sidx}.
 
-  Lemma state_local_update_grow ts t :
-  (● Private ts ⋅ ◯ Private ts, ● Private ts ⋅ ◯ Private ts) ~l~>
-  (● Private (ts ∪ {[ t ]}) ⋅ ◯ Private (ts ∪ {[ t ]}), ● Private (ts ∪ {[ t ]}) ⋅ ◯ Private (ts ∪ {[ t ]})).
+  Lemma state_local_update_lock_Public t :
+    (● Some (Private t) ⋅ ◯ Some (Private t),
+     ● Some (Private t) ⋅ ◯ Some (Private t)) ~l~>
+    (● Some (Public t) ⋅ ◯ Some (Public t),
+     ● Some (Public t) ⋅ ◯ Some (Public t)).
   Proof.
   apply auth_local_update=> //. apply local_update_discrete.
   move=> mz Hval Heq; split; first done.
-  case: mz Hval Heq=> [[ts1|t1|]|] //= Hval Heq.
-  - change (Private ts ⋅ Private ts1) with (state_op_instance (Private ts) (Private ts1)) in Heq.
-    change (Private (ts ∪ {[ t ]}) ⋅ Private ts1) with (state_op_instance (Private (ts ∪ {[ t ]})) (Private ts1)).
-    simpl in *. f_equal. set_solver.
-  - change (Private ts ⋅ Public t1) with (state_op_instance (Private ts) (Public t1)) in Heq.
-    simpl in Heq.
-    by case_bool_decide.
+  case: mz Hval Heq => [[[t1|t1||]|]|] //= Hval Heq;
+    rewrite -!Some_op !state_op /= in Heq *; fold_leibniz;
+    repeat (case_bool_decide; simplify_eq/=); done.
   Qed.
 
-  Lemma state_local_update_lock t :
-    (● Private {[ t ]} ⋅ ◯ Private {[ t ]}, ● Private {[ t ]} ⋅ ◯ Private {[ t ]}) ~l~>
-    (● Public t ⋅ ◯ Public t, ● Public t ⋅ ◯ Public t).
+  Lemma state_local_update_lock_Secret t :
+    (● Some (Private t) ⋅ ◯ Some (Private t),
+     ● Some (Private t) ⋅ ◯ Some (Private t)) ~l~>
+    (● Some Secret ⋅ ◯ Some Secret,
+     ● Some Secret ⋅ ◯ Some Secret).
   Proof.
   apply auth_local_update=> //. apply local_update_discrete.
   move=> mz Hval Heq; split; first done.
-  case: mz Hval Heq=> [[ts1|t1|]|] //= Hval Heq.
-  - change (Private {[ t ]} ⋅ Private ts1) with (state_op_instance (Private {[ t ]}) (Private ts1)) in Heq.
-    change (Public t ⋅ Private ts1) with (state_op_instance (Public t) (Private ts1)).
-    simpl in *. injection Heq as Heq.
-    case_bool_decide; set_solver.
-  - change (Private {[ t ]} ⋅ Public t1) with (state_op_instance (Private {[ t ]}) (Public t1)) in Heq.
-    simpl in Heq.
-    by case_bool_decide.
+  case: mz Hval Heq => [[[t1|t1||]|]|] //= Hval Heq;
+    rewrite -!Some_op !state_op /= in Heq *; fold_leibniz;
+    repeat (case_bool_decide; simplify_eq/=); done.
   Qed.
 
   Lemma state_core_id_local_update (st : state) :
-    (● st ⋅ ◯ st, ● st) ~l~>
-    (● st ⋅ ◯ st, ● st ⋅ ◯ st).
+    (● Some st ⋅ ◯ Some st, ● Some st) ~l~>
+    (● Some st ⋅ ◯ Some st, ● Some st ⋅ ◯ Some st).
   Proof.
   apply core_id_local_update; first apply _.
   by rewrite auth_frag_included.
